WIP

src/ra/ObligationRA.v
@@ -644,6 +644,7 @@ Module ObligationRA.
       iPoseProof (white_split_eq with "H1") as "[H1 H2]".
       iFrame. iModIntro. iExists _. iFrame.
     Qed.
+
   End EDGE.
 
 
@@ -1700,6 +1701,54 @@ Module ObligationRA.
         OwnM (@Regions.nauth_ra (fun i => (S * nat * Ord.t * Qp * nat * Vars i)%type) j).
 
     End SATS.
+
+    Section COLLECT.
+
+      (* Variable (v: index). *)
+      (* Local Notation Var := (Vars v). *)
+
+      Definition collect_tax o : (nat * Ord.t) -> iProp :=
+        fun '(k, c) => white k ((c × Ord.omega) × o)%ord.
+
+      Definition collection_tax k o (l : list (nat * Ord.t)) :=
+        (black k o ∗ Region.sat_list (collect_tax o) l)%I.
+
+      Lemma collect_tax_split o k c :
+        forall o0, (o0 < o)%ord ->
+              collect_tax o (k, c) ⊢ #=> collect_tax o0 (k, c) ∗ white k (c × Ord.omega)%ord.
+      Proof.
+        iIntros (o0 LT) "C". unfold collect_tax.
+        iMod (white_split ((c × Ord.omega) × o0)%ord ((c × Ord.omega) × (Ord.S Ord.O))%ord with "C") as "[C0 C1]".
+        { rewrite <- ClassicJacobsthal.mult_dist. apply Jacobsthal.le_mult_r.
+          rewrite Hessenberg.add_S_r. rewrite Hessenberg.add_O_r. apply Ord.S_supremum; auto.
+        }
+        iModIntro. iFrame. iApply white_eq. 2: iFrame.
+        apply Jacobsthal.mult_1_r.
+      Qed.
+
+      Lemma collect_taxes_split o l :
+        forall o0, (o0 < o)%ord ->
+              Region.sat_list (collect_tax o) l ⊢ #=> Region.sat_list (collect_tax o0) l ∗ tax l.
+      Proof.
+        induction l; iIntros (o0 LT) "C".
+        { ss. }
+        ss. iDestruct "C" as "[T C]". iMod (IHl o0 LT with "C") as "[C T2]". iFrame.
+        destruct a as [k c]. iApply collect_tax_split; eauto.
+      Qed.
+
+      Lemma collection_tax_decr k o l :
+        (collection_tax k o l)
+          -∗
+          (white_one k)
+          -∗
+          (#=> ∃ o', collection_tax k o' l ∗ ⌜(o' < o)%ord⌝ ∗ tax l).
+      Proof.
+        iIntros "[B C] W". iMod (black_white_decr_one with "B W") as "[% [B2 %]]".
+        iExists o0. iFrame. iMod (collect_taxes_split with "C") as "[C T]". eauto.
+        iFrame. iPureIntro. auto.
+      Qed.
+
+    End COLLECT.
 
   End ARROW.
 
